---
title: "GPT helps with Lemma 2.3"
author:
  - "Edward Ionides and Aaron King"
date: September 18, 2025
date-format: long
format:
  pdf

---

**PROMPT**: what is this identity? can you prove it?

\includegraphics[width=5cm]{lem2-3.png}

**UM-GPT**: Let's state the identity and then prove it:

## **The Identity**

$$
\sum_{N=n}^{\infty} \binom{N}{n} a^N = \frac{a^n}{(1-a)^{n+1}}
$$

where \(|a| < 1$.

----

## **Proof**

Let's break the sum down and then manipulate it to get the right-hand side.

### **Step 1: Rewrite the Binomial Coefficient**

Recall that:

$$
\binom{N}{n} = \frac{N!}{n!(N-n)!}
$$

So,

$$
\sum_{N=n}^{\infty} \binom{N}{n} a^N
$$

But let's find a more convenient wayâ€”**Shift index:** Let $M = N - n$, so as $N$ goes from $n$ to $\infty$, $M$ goes from $0$ to $\infty$.

So,

$$
\sum_{N=n}^{\infty} \binom{N}{n} a^N = \sum_{M=0}^{\infty} \binom{M+n}{n} a^{M+n}
$$

$$
= a^n \sum_{M=0}^{\infty} \binom{M+n}{n} a^{M}
$$

----

### **Step 2: Recognize the Generating Function**

Recall the generating function:

$$
\sum_{M=0}^{\infty} \binom{M+n}{n} x^M = \frac{1}{(1-x)^{n+1}}, \quad |x| < 1
$$

Set $x = a$:

$$
\sum_{M=0}^{\infty} \binom{M+n}{n} a^M = \frac{1}{(1-a)^{n+1}}
$$

---

### **Step 3: Multiply by $a^n$**

$$
a^n \sum_{M=0}^{\infty} \binom{M+n}{n} a^{M} = a^n \frac{1}{(1-a)^{n+1}}
$$

---

### **Final Step: Write the Full Identity**

$$
\sum_{N=n}^{\infty} \binom{N}{n} a^N = \frac{a^n}{(1-a)^{n+1}}
$$

---

## **Summary**

This is a binomial sum identity, closely related to the generating function for the sequence $\binom{N+n}{n}$. The proof makes use of index shifting and properties of generating functions.

**If you want more context or a different proof (e.g., combinatorial meaning or induction), just let me know!**
